a

prescan.v
@@ -46,257 +46,280 @@ for (d = 1; d < n; d ∗= 2) {
 }
 barrier(); // ϕspec
 // (iii) compaction if (flag[tid]) out[idx[tid]] = data[tid];
-*)
+ *)
 
 Require Import GPUCSL scan_lib.
 
 Section Prescan.
-Notation Tid := (Var 0).
-Notation In := (Var 1). 
-Notation Sum := (Var 2).
-Notation Pres := (Var 3).
+  Notation Tid := (Var 0).
+  Notation In := (Var 1). 
+  Notation Sum := (Var 2).
+  Notation Pres := (Var 3).
 
-Notation D := (Var 4).
-Notation Offset := (Var 5).
-Notation Tmp1 := (Var 6).
-Notation Tmp2 := (Var 7).
+  Notation D := (Var 4).
+  Notation Offset := (Var 5).
+  Notation Tmp1 := (Var 6).
+  Notation Tmp2 := (Var 7).
 
-Infix "+C" := (Eplus) (at level 50).
-Infix "*C" := (Emult) (at level 40).
-Infix "-C" := (Esub) (at level 50).
-Infix "<C" := (Blt) (at level 70).
+  Infix "+C" := (Eplus) (at level 50).
+  Infix "*C" := (Emult) (at level 40).
+  Infix "-C" := (Esub) (at level 50).
+  Infix "<C" := (Blt) (at level 70).
 
-Notation leftC ARR := (ARR +C Offset *C (Enum 2 *C Tid +C Enum 1) -C Enum 1).
-Notation rightC ARR := (ARR +C Offset *C (Enum 2 *C Tid +C Enum 2) -C Enum 1).
+  Notation leftC ARR := (ARR +C Offset *C (Enum 2 *C Tid +C Enum 1) -C Enum 1).
+  Notation rightC ARR := (ARR +C Offset *C (Enum 2 *C Tid +C Enum 2) -C Enum 1).
 
-Notation Zn := Z.of_nat.
+  Notation Zn := Z.of_nat.
 
-Variable f_ini : nat -> Z.
-Variable ntrd : nat.
+  Variable f_ini : nat -> Z.
+  Variable ntrd : nat.
 
-Hypothesis ntrd_is_p2 : exists e, ntrd = 2 ^ e.
-Lemma ntrd_neq_0 : ntrd <> 0.
-Proof.
-  destruct ntrd_is_p2; rewrite H; apply Nat.pow_nonzero; auto.
-Qed.
+  Hypothesis ntrd_is_p2 : exists e, ntrd = 2 ^ e.
+  Lemma ntrd_neq_0 : ntrd <> 0.
+  Proof.
+    destruct ntrd_is_p2; rewrite H; apply Nat.pow_nonzero; auto.
+  Qed.
 
-Require Import Recdef.
+  Require Import Recdef.
 
-Function rdiv2 n {wf lt n} :=
-  match n with
-    | 0 => 0
-    | _ => if Nat.eq_dec (n mod 2) 0 then S (rdiv2 (n / 2)) else 0
-  end%nat.
-Proof.
-  intros; destruct Nat.eq_dec; try omega.
-  apply Nat.div_lt; omega.
-  apply lt_wf.
-Defined.
+  Function rdiv2 n {wf lt n} :=
+    match n with
+      | 0 => 0
+      | _ => if Nat.eq_dec (n mod 2) 0 then S (rdiv2 (n / 2)) else 0
+    end%nat.
+  Proof.
+    intros; destruct Nat.eq_dec; try omega.
+    apply Nat.div_lt; omega.
+    apply lt_wf.
+  Defined.
 
-Definition upInv (i : nat) :=
-  Ex (offset d : nat) (f : nat -> Z), 
+  Definition upInv (i : nat) :=
+    Ex (offset d : nat) (f : nat -> Z), 
     !(Tid === Zn i) **
-    !(Offset === Zn offset) **
-    !(D === Zn d) **
-    !(pure ((d = 0) /\ (offset = ntrd * 2) \/ (d * offset = ntrd))) **
-    !(pure (forall i, f i = let m := min (2 ^ rdiv2 (i + 1)) offset in
-                      sum_of (i + 1 - m) m f_ini)) **
-    (if lt_dec i (ceil2 d) then is_array Sum (Nat.max 2 offset) f (i * (Nat.max 2 offset)) else emp).
+     !(Offset === Zn offset) **
+     !(D === Zn d) **
+     !(pure ((d = 0) /\ (offset = ntrd * 2) \/ (d * offset = ntrd))) **
+     if lt_dec i (dbl d) then 
+       !(pure (forall i, i < ntrd * 2 ->
+                 f i = let m := min (2 ^ rdiv2 (i + 1)) offset in
+                       sum_of (i + 1 - m) m f_ini)) **
+        (is_array Sum (Nat.max 2 offset) f (i * (Nat.max 2 offset)))
+     else
+       emp.
 
-Definition bspec n :=
-  if Nat.eq_dec n 0 then
-    (MyVector.init (fun i : Fin.t ntrd => 
-       Ex (offset d : nat) (f : nat -> Z), 
-       !(Tid === Zn (nf i)) **
-       !(Offset === Zn offset) **
-       !(D === Zn d) **
-       !(pure ((d = 0) /\ (offset = ntrd * 2) \/ (d * offset = ntrd))) **
-       !(pure (forall i, f i = let m := min (2 ^ rdiv2 (i + 1)) offset in
-                               sum_of (i + 1 - m) m f_ini)) **
-       (if lt_dec (nf i) d then
-          is_array Sum (Nat.max 2 offset) f ((nf i) * (Nat.max 2 offset))
-        else emp)),
-     MyVector.init (fun i : Fin.t ntrd => 
-       Ex (offset d : nat) (f : nat -> Z), 
-       !(Tid === (Zn (nf i))) **
-       !(Offset === Zn offset) **
-       !(D === Zn d) **
-       !(pure ((d = 0) /\ (offset = ntrd * 2) \/ (d * offset = ntrd))) **
-       !(pure (forall i, f i = let m := min (2 ^ rdiv2 (i + 1)) offset in
-                               sum_of (i + 1 - m) m f_ini)) **
-       (if lt_dec (nf i) (ceil2 d) then is_array Sum (offset * 2) f ((nf i) * offset * 2) else emp)))
-  else default ntrd.
+  Definition bspec n :=
+    if Nat.eq_dec n 0 then
+      (MyVector.init (fun i : Fin.t ntrd => 
+         Ex (offset d : nat) (f : nat -> Z), 
+         !(Offset === Zn offset) **
+         !(D === Zn d) **
+         !(pure ((d = 0) /\ (offset = ntrd * 2) \/ (d * offset = ntrd))) **
+         !(pure (0 < d)) **
+         if lt_dec (nf i) (d * 2) then
+              !(pure (forall i, i < ntrd * 2 ->
+                                f i = let m := min (2 ^ rdiv2 (i + 1)) offset in
+                                      sum_of (i + 1 - m) m f_ini)) **
+            is_array Sum (Nat.max 2 offset) f ((nf i) * (Nat.max 2 offset))
+         else emp),
+       MyVector.init (fun i : Fin.t ntrd => 
+         Ex (offset d : nat) (f : nat -> Z), 
+           !(Offset === Zn offset) **
+           !(D === Zn d) **
+           !(pure ((d = 0) /\ (offset = ntrd * 2) \/ (d * offset = ntrd))) **
+           !(pure (0 < d)) **
+           if lt_dec (nf i) d then
+             !(pure (forall i, i < ntrd * 2 ->
+                               f i = let m := min (2 ^ rdiv2 (i + 1)) offset in
+                                     sum_of (i + 1 - m) m f_ini)) **
+              is_array Sum (offset * 2) f ((nf i) * offset * 2)
+           else emp))
+    else default ntrd.
 
-Definition upsweep (i : nat) :=
-  Offset ::= 1%Z ;;
-  D ::= Zn ntrd ;;
-  WhileI (upInv i) (0%Z <C D) (
-    Cbarrier 0 ;;
-    Cif (Tid <C D) (
-      Tmp1 ::= [leftC Sum] ;;
-      Tmp2 ::= [rightC Sum] ;;
-      [rightC Sum] ::= Tmp1 +C Tmp2
-    ) (Cskip) ;;
-    Offset ::= Offset *C 2%Z ;;
+  Definition upsweep (i : nat) :=
+    Offset ::= 1%Z ;;
+    D ::= Zn ntrd ;;
+    WhileI (upInv i) (0%Z <C D) (
+      Cbarrier 0 ;;
+      Cif (Tid <C D) (
+        Tmp1 ::= [leftC Sum] ;;
+        Tmp2 ::= [rightC Sum] ;;
+        [rightC Sum] ::= Tmp1 +C Tmp2
+      ) (Cskip) ;;
+      Offset ::= Offset *C 2%Z ;;
     D ::= D>>1
   ).
 
-Ltac ex_dest_in H id :=
-  lazymatch type of H with
-    | ((Ex _, _) ** _) _ _ => apply ex_lift_l_in in H; destruct H as [id H]
-    | (_ ** (Ex _, _)) _ _ => apply ex_lift_r_in in H; destruct H as [id H]
-end.
-
-(* TODO: ex_lift_rに対応 *)
-Ltac sep_ex :=
-  lazymatch goal with
-    | [ |- ((Ex _, _) ** _) _ _] => apply ex_lift_l
+  Ltac ex_dest_in H id :=
+    lazymatch type of H with
+  | ((Ex _, _) ** _) _ _ => apply ex_lift_l_in in H; destruct H as [id H]
+  | (_ ** (Ex _, _)) _ _ => apply ex_lift_r_in in H; destruct H as [id H]
   end.
 
-Lemma fin_lt (n : nat) (i : Fin.t n) : (nf i) < n.
-Proof.
-  destruct (Fin.to_nat i); simpl; auto.
-Qed.
+  (* TODO: ex_lift_rに対応 *)
+  Ltac sep_ex :=
+    lazymatch goal with
+  | [ |- ((Ex _, _) ** _) _ _] => apply ex_lift_l
+  end.
 
-Lemma is_array_unfold Arr len' f : forall s len,
-  len' < len ->
-  forall stc, 
-    stc ||= is_array Arr len f s <=>
-        is_array Arr len' f s **
-        (Arr +C (Zn (len' + s))%Z -->p (1, f (len' + s))) **
-        is_array Arr (len - len' - 1) f (S (len' + s)).
-Proof.
-  induction len'; intros s len Hlen stc.
-  - destruct len; try omega; simpl.
-    rewrite <-minus_n_O, emp_unit_l; reflexivity.
-  - destruct len; [inversion Hlen|]; simpl.
-    rewrite IHlen'; try omega.
-    rewrite <-plus_n_Sm; simpl; rewrite sep_assoc; autorewrite with sep. reflexivity.
-Qed.
+  Lemma fin_lt (n : nat) (i : Fin.t n) : (nf i) < n.
+  Proof.
+    destruct (Fin.to_nat i); simpl; auto.
+  Qed.
 
-Hint Rewrite Nat2Z.inj_add Nat2Z.inj_mul Nat2Z.inj_sub : sep.
-Arguments div _ _ : simpl never.
-Arguments Nat.max _ _ : simpl never.
+  Lemma is_array_unfold Arr len' f : forall s len,
+    len' < len ->
+    forall stc, 
+      stc ||= is_array Arr len f s <=>
+          is_array Arr len' f s **
+          (Arr +C (Zn (len' + s))%Z -->p (1, f (len' + s))) **
+          is_array Arr (len - len' - 1) f (S (len' + s)).
+  Proof.
+    induction len'; intros s len Hlen stc.
+    - destruct len; try omega; simpl.
+      rewrite <-minus_n_O, emp_unit_l; reflexivity.
+    - destruct len; [inversion Hlen|]; simpl.
+      rewrite IHlen'; try omega.
+      rewrite <-plus_n_Sm; simpl; rewrite sep_assoc; autorewrite with sep. reflexivity.
+  Qed.
 
-Lemma div_pow2 : forall e n m, n * m = 2 ^ e -> exists e1 e2, n = 2 ^ e1 /\ m = 2 ^ e2.
-Proof.
-  induction e; intros n m Hnm.
-  - exists 0, 0; simpl.
-    apply mult_is_one; auto.
-  - rewrite pow_succ_r in Hnm; try omega.
-    assert (n mod 2 = 0 \/ n mod 2 = 1) by (pose proof (Nat.mod_upper_bound n 2); omega).
-    rewrite (Nat.div_mod n 2) in Hnm; auto; auto.
-    destruct H; rewrite H in Hnm.
-    + rewrite <-plus_n_O in Hnm.
-      rewrite <-mult_assoc, Nat.mul_cancel_l in Hnm; auto.
-      apply IHe in Hnm; try omega; destruct Hnm as (e1 & e2 & Hnm); exists (S e1), e2.
-      rewrite (Nat.div_mod n 2), H; auto; simpl. omega.
-    + assert (m mod 2 = 0 \/ m mod 2 = 1) by (pose proof (Nat.mod_upper_bound m 2); omega).
-      rewrite (Nat.div_mod m 2) in Hnm; auto; auto.
-      destruct H0; rewrite H0 in Hnm.
-      rewrite <-plus_n_O in Hnm.
-      rewrite <-mult_comm, <-mult_assoc, Nat.mul_cancel_l in Hnm; auto.
-      apply IHe in Hnm as (e1 & e2 & Hnm); exists e2, (S e1).
-      rewrite (Nat.div_mod m 2), (Nat.div_mod n 2), H, H0; simpl; omega.
-      ring_simplify in Hnm. 
-      cutrewrite (4 * (n / 2) * (m / 2) + 2 * (n / 2) + 2 * (m / 2) + 1 =
-                  2 * (2 * (n / 2) * (m / 2) + (n / 2) + (m / 2)) + 1) in Hnm; [omega|].
-      ring.
-Qed.
+  Hint Rewrite Nat2Z.inj_add Nat2Z.inj_mul Nat2Z.inj_sub : sep.
+  Arguments div _ _ : simpl never.
+  Arguments Nat.max _ _ : simpl never.
 
-Lemma rdiv2_mult (n m : nat) : m <> 0 -> 2 ^ n <= 2 ^ rdiv2 (2 ^ n * m).
-Proof.
-  intros Hm0; remember (2 ^ n * m) as nm eqn:eqnm; revert n m eqnm Hm0; functional induction (rdiv2 nm).
-  - intros; symmetry in eqnm; apply mult_is_O in eqnm; omega.
-  - intros n' m Hnm Hm0.
-    destruct n'; subst; [simpl; autorewrite with sep;
-                         pose proof (Nat.pow_nonzero 2 (rdiv2 (m / 2))); omega|].
-    rewrite !Nat.pow_succ_r', <-Nat.mul_le_mono_pos_l; auto.
-    eapply (IHn _ m); auto.
-    rewrite Nat.pow_succ_r'. 
-    cutrewrite (2 * 2 ^ n' * m = 2 ^ n' * m * 2); [|ring]; rewrite Nat.div_mul; auto.
-  - intros n' m Hnm Hm0.
-    destruct n'; auto; subst.
-    clear e0; rewrite Nat.pow_succ_r' in _x0. rewrite <-mult_assoc, mult_comm in _x0.
-    rewrite  Nat.mod_mul in _x0; omega.
-Qed.
+  Lemma div_pow2 : forall e n m, n * m = 2 ^ e -> exists e1 e2, n = 2 ^ e1 /\ m = 2 ^ e2.
+  Proof.
+    induction e; intros n m Hnm.
+    - exists 0, 0; simpl.
+      apply mult_is_one; auto.
+    - rewrite pow_succ_r in Hnm; try omega.
+      assert (n mod 2 = 0 \/ n mod 2 = 1) by (pose proof (Nat.mod_upper_bound n 2); omega).
+      rewrite (Nat.div_mod n 2) in Hnm; auto; auto.
+      destruct H; rewrite H in Hnm.
+      + rewrite <-plus_n_O in Hnm.
+        rewrite <-mult_assoc, Nat.mul_cancel_l in Hnm; auto.
+        apply IHe in Hnm; try omega; destruct Hnm as (e1 & e2 & Hnm); exists (S e1), e2.
+        rewrite (Nat.div_mod n 2), H; auto; simpl. omega.
+      + assert (m mod 2 = 0 \/ m mod 2 = 1) by (pose proof (Nat.mod_upper_bound m 2); omega).
+        rewrite (Nat.div_mod m 2) in Hnm; auto; auto.
+        destruct H0; rewrite H0 in Hnm.
+        rewrite <-plus_n_O in Hnm.
+        rewrite <-mult_comm, <-mult_assoc, Nat.mul_cancel_l in Hnm; auto.
+        apply IHe in Hnm as (e1 & e2 & Hnm); exists e2, (S e1).
+        rewrite (Nat.div_mod m 2), (Nat.div_mod n 2), H, H0; simpl; omega.
+        ring_simplify in Hnm. 
+        cutrewrite (4 * (n / 2) * (m / 2) + 2 * (n / 2) + 2 * (m / 2) + 1 =
+                    2 * (2 * (n / 2) * (m / 2) + (n / 2) + (m / 2)) + 1) in Hnm; [omega|].
+        ring.
+  Qed.
+
+  Lemma rdiv2_mult (n m : nat) : m <> 0 -> 2 ^ n <= 2 ^ rdiv2 (2 ^ n * m).
+  Proof.
+    intros Hm0; remember (2 ^ n * m) as nm eqn:eqnm; revert n m eqnm Hm0; functional induction (rdiv2 nm).
+    - intros; symmetry in eqnm; apply mult_is_O in eqnm; omega.
+    - intros n' m Hnm Hm0.
+      destruct n'; subst; [simpl; autorewrite with sep;
+                           pose proof (Nat.pow_nonzero 2 (rdiv2 (m / 2))); omega|].
+      rewrite !Nat.pow_succ_r', <-Nat.mul_le_mono_pos_l; auto.
+      eapply (IHn _ m); auto.
+      rewrite Nat.pow_succ_r'. 
+      cutrewrite (2 * 2 ^ n' * m = 2 ^ n' * m * 2); [|ring]; rewrite Nat.div_mul; auto.
+    - intros n' m Hnm Hm0.
+      destruct n'; auto; subst.
+      clear e0; rewrite Nat.pow_succ_r' in _x0. rewrite <-mult_assoc, mult_comm in _x0.
+      rewrite  Nat.mod_mul in _x0; omega.
+  Qed.
 
 
-Lemma is_array_unfold' Arr len f : forall s,
-  0 < len ->
-  forall stc, 
-    stc ||= is_array Arr len f s <=>
-        is_array Arr (len - 1) f s **
-        (Arr +C (Zn (s + len - 1)) -->p (1, f (s + len - 1))).
-Proof.
-  induction len; intros s Hlen stc; try omega.
-  destruct len.
-  - simpl; rewrite <-plus_n_Sm, <-plus_n_O; simpl;
-    rewrite emp_unit_l, emp_unit_r, <-minus_n_O; reflexivity.
-  - remember (S len); simpl.
-    rewrite IHlen; try omega.
-    subst; simpl; rewrite <-!minus_n_O.
-    rewrite <-(plus_n_Sm s (S len)); simpl; rewrite <-minus_n_O, sep_assoc. reflexivity.
-Qed.
+  Lemma is_array_unfold' Arr len f : forall s,
+    0 < len ->
+    forall stc, 
+      stc ||= is_array Arr len f s <=>
+          is_array Arr (len - 1) f s **
+          (Arr +C (Zn (s + len - 1)) -->p (1, f (s + len - 1))).
+  Proof.
+    induction len; intros s Hlen stc; try omega.
+    destruct len.
+    - simpl; rewrite <-plus_n_Sm, <-plus_n_O; simpl;
+      rewrite emp_unit_l, emp_unit_r, <-minus_n_O; reflexivity.
+    - remember (S len); simpl.
+      rewrite IHlen; try omega.
+      subst; simpl; rewrite <-!minus_n_O.
+      rewrite <-(plus_n_Sm s (S len)); simpl; rewrite <-minus_n_O, sep_assoc. reflexivity.
+  Qed.
 
-Hint Resolve fin_lt.
+  Hint Resolve fin_lt.
 
-Lemma upsweep_correct (i : Fin.t ntrd) :
-  CSL bspec i 
-      (is_array Sum 1 f_ini (nf i))
-      (upsweep (nf i))
-      (if Nat.eq_dec (nf i) 0 then 
-         Ex f, 
-           !(pure (forall i, f i = let m := 2 ^ rdiv2 i in sum_of (i + 1 - m) m f)) ** 
-           is_array Sum (ntrd * 2) f 0
-       else emp).
-Proof.
-  pose proof ntrd_neq_0 as ntrd_neq_0.
-  unfold upsweep.
-  eapply rule_seq; [hoare_forward; intros ? ? [v H] | ].
-  { remember 1 in H. subA_normalize_in H. simpl in H. subst; exact H. }
-  eapply rule_seq; [hoare_forward; intros ? ? [v H] | ].
-  { remember 1 in H; subA_normalize_in H. simpl in H. subst. exact H. }
-  hoare_forward.
-  Hint Unfold bspec upInv.
-  
-  eapply rule_seq; [hoare_forward|].
-  { intros s h H.
-    ex_dest_in H offset; ex_dest_in H d; ex_dest_in H f.
-    sep_ex; exists offset; sep_ex; exists d; sep_ex; exists f.
-    sep_split_in H; sep_normal; sep_split; eauto.
-    change_in H.
-    { unfold_pures; unfold ceil2 in H; destruct Nat.eq_dec; try omega.
-      exact H. }
-    sep_rewrite_in_r emp_unit_r H. apply H. }
-
-  { autounfold; simpl; intros ? ? H; rewrite MyVector.init_spec in H. 
-    sep_rewrite_in emp_unit_r H. exact H. }
-  
-  repeat hoare_forward; revert x x0 x1; intros offset d fc.
-  eapply rule_seq. eapply rule_if_disj.
-  
-  { eapply Hbackward. 
-    Focus 2.
-    { intros s h H; sep_normal_in H; sep_split_in H.
+  Lemma upsweep_correct (i : Fin.t ntrd) :
+    CSL bspec i 
+        (is_array Sum 2 f_ini (nf i * 2) ** !(Tid === Zn (nf i)))
+        (upsweep (nf i))
+        (if Nat.eq_dec (nf i) 0 then 
+           Ex f, 
+           !(pure (forall i, i < ntrd * 2 ->
+                             f i = let m := 2 ^ rdiv2 (i + 1) in sum_of (i + 1 - m) m f_ini)) ** 
+            is_array Sum (ntrd * 2) f 0
+         else emp).
+  Proof.
+    pose proof ntrd_neq_0 as ntrd_neq_0.
+    unfold upsweep.
+    (* the 1st command *)
+    eapply rule_seq; [hoare_forward; intros ? ? [v H] | ].
+    { remember 1 in H. subA_normalize_in H. simpl in H. subst; exact H. }
+    (* the snd command *)
+    eapply rule_seq; [hoare_forward; intros ? ? [v H] | ].
+    { remember 1 in H; subA_normalize_in H. simpl in H. subst. exact H. }
+    hoare_forward.
+    Hint Unfold bspec upInv.
+    
+    (* loop body *)
+    (* barrier *)
+    eapply rule_seq; [hoare_forward|].
+    (* the barrier precondition holds *)
+    { intros s h H.
+      ex_dest_in H offset; ex_dest_in H d; ex_dest_in H f.
+      sep_ex; exists offset; sep_ex; exists d; sep_ex; exists f.
+      sep_split_in H. sep_normal; sep_split; eauto.
+      { unfold_pures; unfold_conn; omega. }
       change_in H.
-      { unfold_pures.
-        Lemma ceil2_leq (n : nat) : n <= ceil2 n.
-        Proof.
-          unfold ceil2; destruct Nat.eq_dec; omega.
-        Qed.
-        destruct lt_dec.
-        2: rewrite HP, HP1 in l; rewrite <-Nat2Z.inj_lt in l; pose proof (ceil2_leq d); omega.
-        assert (Hoff0 : offset <> 0) by (intros Hc; subst; destruct HP2; omega).
-        sep_rewrite_in is_array_unfold' H; try omega.
-        sep_rewrite_in is_array_unfold H. 
-        2: instantiate (1 := offset - 1); omega.
-        cutrewrite (offset - 1 + nf i * offset * 2 = offset * (2 * nf i + 1) - 1) in H.
-        Focus 2.
-        { cutrewrite (offset * (2 * nf i + 1) = nf i * offset * 2 + offset); [|ring]. 
-          generalize (nf i * offset * 2); intros; omega. } Unfocus.
-        cutrewrite (nf i * offset * 2 + offset * 2 - 1 = offset * (2 * nf i + 2) - 1) in H.
-        Focus 2.
+      { unfold_pures; unfold dbl in H; destruct Nat.eq_dec; try omega.
+        exact H. }
+      clear HP HP1 HP2 HP3.
+      sep_combine_in H. apply H. }
+    
+    (* transform the barrier postcondition *)
+    { autounfold; simpl; intros ? ? H; rewrite MyVector.init_spec in H.
+      ex_dest_in H o; ex_dest_in H d; ex_dest_in H f.
+      sep_normal_in H.
+      ex_intro f H; ex_intro d H; ex_intro o H; simpl in H.
+      exact H. }
+    
+    repeat hoare_forward; revert x x0 x1; intros offset d fc.
+    eapply rule_seq. eapply rule_if_disj.
+    
+    (* then case of the branch *)
+    { eapply Hbackward. 
+      (* unfold the is_array predicate *)
+      Focus 2.
+      { intros s h H; sep_normal_in H; sep_split_in H.
+        change_in H.
+        { unfold_pures.
+          Lemma ceil2_leq (n : nat) : n <= ceil2 n.
+          Proof.
+            unfold ceil2; destruct Nat.eq_dec; omega.
+          Qed.
+          destruct lt_dec.
+          2: rewrite HP0, HP3 in l; rewrite <-Nat2Z.inj_lt in l; pose proof (ceil2_leq d);
+             apply n in l; destruct l.
+          assert (Hoff0 : offset <> 0) by (intros Hc; subst; destruct HP2; omega).
+          sep_rewrite_in is_array_unfold' H; try omega.
+          sep_rewrite_in is_array_unfold H. 
+          2: instantiate (1 := offset - 1); omega.
+          cutrewrite (offset - 1 + nf i * offset * 2 = offset * (2 * nf i + 1) - 1) in H.
+          Focus 2.
+          { cutrewrite (offset * (2 * nf i + 1) = nf i * offset * 2 + offset); [|ring]. 
+            generalize (nf i * offset * 2); intros; omega. } Unfocus.
+          cutrewrite (nf i * offset * 2 + offset * 2 - 1 = offset * (2 * nf i + 2) - 1) in H.
+          Focus 2.
         { cutrewrite (offset * (2 * nf i + 2) = nf i * offset * 2 + offset * 2); [|ring].
           omega. } Unfocus.
 
@@ -309,82 +332,486 @@ Proof.
         assert ((Sum +C (Zn offset * (Zn 2 * Zn (nf i) + Zn 2) - Zn 1)%Z ===
                  Sum +C (Offset *C (2 *C Tid +C 2) -C 1)) s emp_ph)%Z.
         { Arguments Z.mul _ _ : simpl never.
-          unfold_conn. simpl. congruence. }
-        sep_normal_in H. sep_lift_in H 3.
+          unfold_conn. simpl.  repeat f_equal; auto. }
+        sep_normal_in H. sep_lift_in H 4.
         sep_rewrite_in (mps_eq1) H; [|apply H1].
         exact H. }
-      (* Arguments Z.add _ _ : simpl never. *)
-      (* Arguments Z.mul _ _ : simpl never. *)
-      (* Arguments plus : simpl never. *)
-      (* Arguments mult : simpl never. *)
       sep_combine_in H; exact H. } Unfocus.
+    (* execute rest of commands *)
     eapply rule_seq; [hoare_forward; intros ? ? H; exact H |].
     eapply rule_seq; [hoare_forward; intros ? ? H; exact H |].
     hoare_forward; intros ? ? H; exact H. }
 
-  apply rule_skip.
-  eapply Hforward.
-  apply (rule_disj (Q1 := (upInv (nf i))) (Q2 := (upInv (nf i)))).  
-  3: intros s h [H1 | H2]; eauto.
-  eapply rule_seq; [hoare_forward; intros s h [v H]; subA_normalize_in H; ex_intro v H; simpl in H; exact H | ].
-  repeat hoare_forward.
-  intros s h [v H]; subA_normalize_in H. simpl in H; sep_split_in H.
-  unfold_pures; subst; autorewrite with sep in *.
-  exists (offset * 2), (d / 2).
-  exists (fun x => if Nat.eq_dec ((x + 1) mod (offset * 2)) 0 then
+    (* else case *)
+    apply rule_skip.
+
+    (* rest of commands *)
+    eapply Hforward.
+    apply (rule_disj (Q1 := (upInv (nf i))) (Q2 := (upInv (nf i)))).  
+    3: intros s h [H1 | H2]; eauto.
+
+    (* rest of commands (then case) *)
+    eapply rule_seq; [hoare_forward; intros s h [v H]; subA_normalize_in H; ex_intro v H; simpl in H; exact H | ].
+    (* the loop invariant is preserved *)
+    repeat hoare_forward.
+    intros s h [v H]; subA_normalize_in H. simpl in H; sep_split_in H.
+    unfold_pures; subst; autorewrite with sep in *.
+    exists (offset * 2), (d / 2).
+    set (fc' := fun x => if Nat.eq_dec ((x + 1) mod (offset * 2)) 0 then
                      (fc x + fc (x - offset)%nat)%Z
                    else fc x).
-  sep_split; autorewrite with sep in *; eauto.
-  - unfold_conn; rewrite HP3 in *; rewrite <-Nat2Z.inj_lt in l. 
-    destruct HP6; try omega.
-    pose proof (Nat.div_mod d 2).
-    destruct ntrd_is_p2 as [e ntrd_2e]; rewrite ntrd_2e in H0; 
-    pose proof (div_pow2 _ _ _ H0) as (e1 & e2 & Hdo).
-    destruct e1; destruct Hdo; subst; [simpl; unfold div; simpl|].
-    left; split; eauto; simpl in H0; omega.
-    autorewrite with sep; auto.
-    rewrite pow_succ_r in H0; try omega; rewrite <-H0; right; ring.
-  - unfold_conn; intros ix.
-    destruct Nat.eq_dec; rewrite !HP7.
-    + assert (offset <> 0) by (destruct offset; destruct HP6; omega).
-      rewrite (Nat.div_mod (ix + 1) (offset * 2)), e; try omega; autorewrite with sep.
+    exists fc'.
+    destruct lt_dec; try omega.
+
+    Focus 2.
+    { rewrite HP7 in l; rewrite <-Nat2Z.inj_lt in l.
+      destruct HP5; try omega.
+      destruct ntrd_is_p2 as [? Hntrd]; rewrite Hntrd in H0; apply div_pow2 in H0 as (? & ? & ? & ?).
+      subst; rewrite dbl_inv in n. tauto. } Unfocus.
+
+    sep_split; autorewrite with sep in *; eauto.
+    - unfold_conn; rewrite HP7 in *; rewrite <-Nat2Z.inj_lt in l. 
+      destruct HP5; try omega.
+      pose proof (Nat.div_mod d 2).
+      destruct ntrd_is_p2 as [e ntrd_2e]; rewrite ntrd_2e in H0; 
+      pose proof (div_pow2 _ _ _ H0) as (e1 & e2 & Hdo).
+      destruct e1; destruct Hdo; subst; [simpl; unfold div; simpl|].
+      left; split; eauto; simpl in H0; omega.
+      autorewrite with sep; auto.
+      rewrite pow_succ_r in H0; try omega; rewrite <-H0; right; ring.
+    - unfold_conn; intros ix Hix; unfold fc' in *.
+      destruct Nat.eq_dec; rewrite !HP9; try omega.
+      + assert (offset <> 0) by (destruct offset; destruct HP6; omega).
+        rewrite (Nat.div_mod (ix + 1) (offset * 2)), e; try omega; autorewrite with sep.
+        
+        assert (exists e, offset = 2 ^ e) as [eoff Hoff].
+        { destruct HP5 as [[? ?]|?]; destruct ntrd_is_p2 as [? ?].
+          - subst; exists (S x); simpl; omega.
+          - subst. apply div_pow2 in H2; destruct H2 as [? [? [? ?]]]; eexists; eauto. }
+        assert ((ix + 1) / (2 ^ eoff * 2) <> 0).
+        { rewrite Nat.div_small_iff; try omega.
+          intros Hlt; rewrite Nat.mod_small in e; auto; omega. }
+        assert (exists k, ix + 1 = 2 ^ eoff * 2 * k /\ k <> 0) as [kix [Hix1 ?]].
+        { rewrite (Nat.div_mod (ix + 1) (2 ^ eoff * 2)); try omega; eexists; split.
+          subst; rewrite e, <-plus_n_O. reflexivity.
+          auto. }
+        subst. rewrite Nat.min_r.
+        2: rewrite <-mult_assoc; apply rdiv2_mult; omega.
+        assert (2 ^eoff <= ix).
+        { cutrewrite (ix = 2 ^ eoff * 2 * kix-1); [|omega].
+          rewrite (mult_comm _ 2); simpl; autorewrite with sep.
+          destruct kix; rewrite mult_comm; simpl; try omega.
+          generalize (2 ^ eoff) H0; intros; destruct n; simpl. omega.
+          generalize (kix * S (n + S n)); intros; omega. }
+        rewrite <-Nat.add_sub_swap; auto.
+        rewrite Hix1.
+        cutrewrite (2 ^ eoff * 2 * kix - 2 ^ eoff = 2 ^ eoff * (2 * kix - 1)); [|].
+        2: rewrite mult_minus_distr_l, mult_assoc, mult_1_r; auto.
+        rewrite Nat.min_r; [|apply rdiv2_mult; omega].
+        rewrite Nat.min_r; [|rewrite (mult_comm (2 ^ eoff) 2), <-Nat.pow_succ_r'; apply rdiv2_mult].
+        2: rewrite mult_comm, Nat.div_mul; auto.
+        rewrite (mult_comm (2 ^ eoff * 2) kix), Nat.div_mul; try omega.
+        cutrewrite (2 ^ eoff * (2 * kix - 1) - 2 ^ eoff = 2 ^ eoff * 2 * kix - 2 ^ eoff * 2).
+        2: rewrite mult_minus_distr_l, <-Nat.sub_add_distr; f_equal; ring.
+        cutrewrite (2 ^ eoff * 2 = 2 ^ eoff + 2 ^ eoff); [|omega].
+        rewrite sum_of_concat, Z.add_comm; f_equal.
+        f_equal. 
+        rewrite Nat.sub_add_distr, <-le_plus_minus; auto.
+        destruct kix; simpl; try omega; rewrite mult_comm; simpl. generalize (kix * (2 ^ eoff + 2 ^ eoff)); intros; omega.
+      + cutrewrite (min (2 ^ rdiv2 (ix + 1)) offset = min (2 ^ rdiv2 (ix + 1)) (offset * 2)); auto.
+        destruct ntrd_is_p2 as [en Hen]; rewrite Hen in HP5.
+        destruct HP5 as [? | HP5]; try omega; apply div_pow2 in HP5 as (eoff & ed & Heoff & Hed);subst.
+        assert (Hle : rdiv2 (ix + 1) <= ed).
+        2: apply (Nat.pow_le_mono_r 2) in Hle; try omega; rewrite !Min.min_l; omega.
+        apply Nat.nlt_ge; intros Hc; unfold lt in Hc.
+        
+        Lemma rdiv2_div (x y : nat) : x <= rdiv2 y -> y mod (2 ^ x) = 0.
+        Proof.
+          revert x; functional induction (rdiv2 y); intros x Hx.
+          - apply Nat.mod_0_l, Nat.pow_nonzero; omega.
+          - destruct x; [simpl; auto|].
+            clear e0; rewrite <-Nat.div_exact in _x0; auto; rewrite Nat.pow_succ_r', _x0.
+            rewrite Nat.mul_mod_distr_l; auto; rewrite IHn; omega.
+          - assert (x = 0) by omega; subst; simpl; auto.
+        Qed.
+        
+        apply rdiv2_div in Hc; rewrite Nat.pow_succ_r', mult_comm in Hc; auto.
+    - destruct HP5 as [? | HP5]; try omega.
+      assert (offset <> 0) by (destruct offset; rewrite mult_comm in HP5; omega).
+      cutrewrite (offset * 2 - 1 - (offset - 1) = offset) in H; [|omega].
+      rewrite !mult_plus_distr_l, mult_1_r, minus_Sn_m in H; [|destruct offset; try omega; generalize (S offset * nf i); intros; try omega].
+      simpl in H; rewrite <-minus_n_O in H; cutrewrite (offset * nf i + offset * nf i = offset * nf i * 2) in H; [|omega].
+      rewrite (mult_comm (nf i) offset) in H.
+      assert (Heq1 : ((Sum +C Zn offset *C (2%Z *C Tid +C 2%Z)) -C 1%Z ===
+                                                                   Sum +C Zn (offset * nf i * 2 + offset + offset - 1)) s emp_ph).
+      { unfold_conn; repeat autorewrite with sep; [|destruct offset; try omega; generalize (S offset * nf i * 2); intros; omega]; simpl.
+        rewrite HP7. rewrite Z.add_sub_assoc. 
+        ring_simplify. reflexivity. }
+      sep_rewrite_in mps_eq1 H; [|exact Heq1]; clear Heq1.
+      assert (Heq1 : ((Sum +C Zn offset *C (2%Z *C Tid +C 1%Z)) -C 1%Z ===
+                                                                   Sum +C Zn (offset * nf i * 2 + offset - 1)) s emp_ph).
+      { unfold_conn; repeat autorewrite with sep; [|destruct offset; try omega; generalize (S offset * nf i * 2); intros; omega]; simpl.
+        rewrite HP7; ring_simplify; reflexivity. }
+      sep_lift_in H 1; sep_rewrite_in mps_eq1 H; [|exact Heq1]; clear Heq1.
+      (* sep_lift_in H 2. sep_lift_in H 3. sep_lift_in H 3. *)
+      
+      Lemma is_array_change (e : exp) (f1 f2 : nat -> Z) n :
+        forall s, (forall x, x < n -> f1 (x + s) = f2(x + s)) ->
+                  forall stc,
+                    stc ||= is_array e n f1 s <=> is_array e n f2 s.
+      Proof.
+        induction n; simpl; intros s Hf; try reflexivity.
+        intros stc; rewrite IHn.
+        cutrewrite (f1 s = f2 s); [reflexivity|].
+        pose proof (Hf 0); rewrite plus_O_n in H; rewrite H; omega.
+        intros x Hx; rewrite <-Nat.add_succ_comm; apply Hf; omega.
+      Qed.
+      assert (Heq :fc (offset * nf i * 2 + offset - 1) =
+                   fc' (offset * nf i * 2 + offset - 1)); [|rewrite Heq in H; clear Heq].
+      unfold fc'; destruct Nat.eq_dec; auto.
+      cutrewrite (offset * nf i * 2 + offset - 1 + 1 = offset * 1 + nf i * (offset * 2)) in e.
+      rewrite Nat.mod_add, Nat.mul_mod_distr_l in e; simpl in e; try omega.
+      rewrite <-Nat.add_sub_swap; try omega. 
+      2: destruct offset; try omega; generalize (S offset * nf i * 2); intros; try omega.
+      rewrite Nat.add_sub; ring.
+      sep_rewrite_in (is_array_change Sum fc fc') H.
+      Focus 2.
+      { intros x Hx; unfold fc'; destruct Nat.eq_dec; auto.
+        cutrewrite (x + offset * nf i * 2 + 1 = x + 1 + nf i * (offset * 2)) in e; [|ring].
+        rewrite Nat.mod_add, <-Nat.div_exact in e; try omega.
+        destruct ((x + 1) / (offset * 2)); rewrite (mult_comm (offset * 2)) in e; simpl in e; try omega.
+        generalize (n * (offset * 2)) e; intros; omega. } Unfocus.
+      sep_rewrite_in (is_array_change Sum fc fc') H.
+      Focus 2.
+      { intros x Hx; unfold fc'; destruct Nat.eq_dec; auto.
+        cutrewrite (x + (offset * nf i * 2 + offset) + 1 = offset + x + 1 + nf i * (offset * 2)) in e; [|ring].
+        rewrite Nat.mod_add, <-Nat.div_exact in e; try omega.
+        destruct ((offset + x + 1) / (offset * 2)); rewrite (mult_comm (offset * 2)) in e; simpl in e; try omega.
+        generalize (n * (offset * 2)) e; intros; omega. } Unfocus.
+      assert (Heq : (Tmp1 +C Tmp2 === fc' (offset * nf i * 2 + offset + offset - 1)) s emp_ph).
+      { unfold_conn; simpl; rewrite HP1, HP2; unfold fc'.
+        cutrewrite (offset * nf i * 2 + offset + offset - 1 + 1 = 
+                    (nf i + 1) * (offset * 2)).
+        rewrite Nat.mod_mul; simpl; try omega; rewrite Z.add_comm; do 2 f_equal.
+        f_equal; ring.
+        rewrite <-Nat.sub_add_distr, (plus_comm 1 offset), Nat.sub_add_distr.
+        f_equal; rewrite Nat.add_sub; ring.
+        rewrite Nat.sub_add; [ring|].
+        generalize (offset * nf i * 2); intros; omega. }
+      sep_lift_in H 1; sep_rewrite_in (mps_eq2) H; [|exact Heq].
+      sep_lift_in H 1. sep_lift_in H 2. sep_lift_in H 3. sep_lift_in H 3.
+      sep_rewrite_in_r (is_array_unfold') H; try omega.
+      sep_lift_in H 1. sep_lift_in H 2. 
+      sep_rewrite_in_r (is_array_unfold') H; try omega.
+      
+      rewrite Nat.max_r; try omega.
     
+      Lemma is_array_concat e f len1 len2 : forall s stc,
+        stc||=
+           is_array e len1 f s ** is_array e len2 f (s + len1) <=>
+           is_array e (len1 + len2) f s.
+      Proof.
+        induction len1; simpl.
+        - intros; rewrite emp_unit_l, <-plus_n_O; reflexivity.
+        - intros. rewrite <-Nat.add_succ_comm, <-sep_assoc, IHlen1; reflexivity.
+      Qed.
+
+      sep_rewrite_in is_array_concat H.
+      cutrewrite (offset + offset = offset * 2) in H; [|ring].
+      cutrewrite (offset * nf i * 2 =  nf i * (offset * 2)) in H; [auto|ring].
+    - (* rest of commands (else case) *)
+      eapply Hbackward.
+      (* in this case, thread does not have any heap resources *)
+      Focus 2.
+      { intros s h H; sep_split_in H.
+        change_in H.
+        { unfold_pures.
+          destruct lt_dec .
+          rewrite HP4, HP1, <-Nat2Z.inj_lt in n; apply n in l; destruct l.
+          exact H.  }
+        sep_combine_in H. exact H. } Unfocus.
+      
+      (* execute rest of commands *)
+      eapply rule_seq; [hoare_forward; intros s h [v H]; subA_normalize_in H; ex_intro v H; exact H|].
+      simpl; repeat hoare_forward. 
+      intros s h [v H]; subA_normalize_in H. simpl in H.
+      sep_split_in H. unfold upInv; unfold_pures.
+      exists (2 * offset), (d /2), fc.
+      destruct ntrd_is_p2 as [en Hen].
+      destruct HP4 as [[? ?] | HP4]; [subst; simpl in *; try omega|].
+      rewrite Hen in HP4; destruct (div_pow2 _ _ _ HP4) as (ed & eoff & Hed & Heoff).
+      autorewrite with sep in *; try omega; sep_split;
+      try now (unfold_conn; simpl; omega || congruence || eauto); eauto.
+      + destruct ed; [left; simpl; auto|].
+        * subst. split. cbv. auto. simpl in HP4. omega.
+        * subst. right. autorewrite with sep; auto.
+          rewrite <-HP4. rewrite Nat.pow_succ_r'. ring.
+      + subst; rewrite dbl_inv.
+        destruct lt_dec; rewrite HP6, <-Nat2Z.inj_lt in *; try tauto.
+    - unfold upInv; intros s h H.
+      ex_dest_in H offset; ex_dest_in H d; ex_dest_in H f.
+      sep_split_in H.
+      unfold_pures.
+      assert (d = 0); [|subst].
+      { apply Nat2Z.inj; rewrite <-HP2; simpl; omega. }
+      unfold dbl in H; simpl in H.
+      destruct lt_dec, Nat.eq_dec; try omega; sep_split_in H; unfold_pures.
+      exists f; unfold_pures.
+      + sep_split.
+        unfold_conn; intros; rewrite HP4; try omega.
+        rewrite Min.min_l; eauto.
+      
+        Lemma rdiv2_eq n : n <> 0 -> exists m, n = 2 ^ rdiv2 n * m /\ m mod 2 = 1.
+        Proof.
+          intros; functional induction (rdiv2 n); try omega.
+          - clear e0; rewrite <-Nat.div_exact in _x0; try omega.
+            assert (n / 2 <> 0) by (rewrite mult_comm in _x0; rewrite _x0, Nat.div_mul; try omega).
+            apply IHn0 in H0 as (m & H1 & H2).
+            exists m; rewrite Nat.pow_succ_r', <-mult_assoc, <-H1; split; auto.
+          - exists n; split; [simpl; omega |].
+                   assert(n mod 2 = 0 \/ n mod 2 = 1).
+                   pose proof (Nat.mod_upper_bound n 2). omega.
+                   destruct H0; omega. 
+        Qed.
+        destruct HP3 as [[_ HP3] | ]; try omega; subst.
+      
+        Lemma rdiv2_leq (i n e : nat) : 
+          n = 2 ^ e -> i <= n -> 2 ^ rdiv2 i <= n.
+        Proof.
+          assert (i = 0 \/ i <> 0) as [H | H] by omega.
+          - subst; simpl; intros; subst.
+            pose proof (Nat.pow_nonzero 2 e); omega.
+          - destruct (rdiv2_eq i H) as [m [Him1 Him2]]; intros; subst n; rewrite Him1 in H1.
+            rewrite mult_comm in H1; destruct m; simpl in *; try omega.
+            generalize (m * 2 ^ rdiv2 i) H1; intros.  omega.
+        Qed.
+
+        destruct ntrd_is_p2 as [en Hen]; rewrite Hen.
+        rewrite mult_comm, <-Nat.pow_succ_r'.
+        eapply rdiv2_leq; eauto. simpl. omega.
+      
+        rewrite e in H; simpl in H.
+        destruct HP3 as [[_ HP3] | ]; try omega; subst.
+        rewrite Nat.max_r in H; eauto.
+        omega.
+
+      + apply H.
+    - intros s h H; sep_split_in H; unfold upInv.
+      unfold_pures.
+      exists 1, ntrd, f_ini; sep_split; auto.
+      unfold_conn; simpl.
+      omega.
+      
+      unfold dbl; destruct Nat.eq_dec; try omega.
+      pose proof (fin_lt ntrd i).
+      destruct lt_dec; try omega.
+      sep_split; [unfold_conn|].
+      intros i0.
+      rewrite Nat.min_r, Nat.add_sub; simpl; try omega.
+      pose proof (Nat.pow_nonzero 2 (rdiv2 (i0 + 1))); try omega.
+      rewrite Nat.max_l; eauto.
+  Qed.
+  Import Bdiv.
+
+  Lemma bspec0_preserved : 
+    Aistar_v (fst (bspec 0)) |= Aistar_v (snd (bspec 0)).
+  Proof.
+    unfold bspec; simpl. intros s h H.
+    apply sc_v2l in H.
+    rewrite (vec_to_list_init0 _ emp) in H.
+    erewrite ls_init_eq0 in H.
+    Focus 2.
+    { intros i Hi.
+      destruct (Fin.of_nat i ntrd) as [|Hex] eqn:Heq; [|destruct Hex; omega].
+      rewrite (Fin_nat_inv Heq). reflexivity. } Unfocus.
+  
+    apply sc_v2l.
+    rewrite (vec_to_list_init0 _ emp).
+    erewrite ls_init_eq0.
+    Focus 2.
+    { intros i iH.
+      destruct (Fin.of_nat i ntrd) as [|Hex] eqn:Heq; [|destruct Hex; omega].
+      rewrite (Fin_nat_inv Heq). reflexivity. } Unfocus.
     
-      assert (exists e, offset = 2 ^ e) as [eoff Hoff].
-      { destruct HP6 as [[? ?]|?]; destruct ntrd_is_p2 as [? ?].
-        - subst; exists (S x); simpl; omega.
-        - subst. apply div_pow2 in H2; destruct H2 as [? [? [? ?]]]; eexists; eauto. }
-      assert ((ix + 1) / (2 ^ eoff * 2) <> 0).
-      { rewrite Nat.div_small_iff; try omega.
-        intros Hlt; rewrite Nat.mod_small in e; auto; omega. }
-      assert (exists k, ix + 1 = 2 ^ eoff * 2 * k /\ k <> 0) as [kix [Hix1 ?]].
-      { rewrite (Nat.div_mod (ix + 1) (2 ^ eoff * 2)); try omega; eexists; split.
-        subst; rewrite e, <-plus_n_O. reflexivity.
-        auto. }
-      subst. rewrite Nat.min_r.
-      2: rewrite <-mult_assoc; apply rdiv2_mult; omega.
-      assert (2 ^eoff <= ix).
-      { cutrewrite (ix = 2 ^ eoff * 2 * kix-1); [|omega].
-        rewrite (mult_comm _ 2); simpl; autorewrite with sep.
-        destruct kix; rewrite mult_comm; simpl; try omega.
-        generalize (2 ^ eoff) H0; intros; destruct n; simpl. omega.
-        generalize (kix * S (n + S n)); intros; omega. }
-      rewrite <-Nat.add_sub_swap; auto.
-      rewrite Hix1.
-      cutrewrite (2 ^ eoff * 2 * kix - 2 ^ eoff = 2 ^ eoff * (2 * kix - 1)); [|].
-      2: rewrite mult_minus_distr_l, mult_assoc, mult_1_r; auto.
-      rewrite Nat.min_r; [|apply rdiv2_mult; omega].
-      rewrite Nat.min_r; [|rewrite (mult_comm (2 ^ eoff) 2), <-Nat.pow_succ_r'; apply rdiv2_mult].
-      2: rewrite mult_comm, Nat.div_mul; auto.
-      rewrite (mult_comm (2 ^ eoff * 2) kix), Nat.div_mul; try omega.
-      cutrewrite (2 ^ eoff * (2 * kix - 1) - 2 ^ eoff = 2 ^ eoff * 2 * kix - 2 ^ eoff * 2).
-      2: rewrite mult_minus_distr_l, <-Nat.sub_add_distr; f_equal; ring.
-      cutrewrite (2 ^ eoff * 2 = 2 ^ eoff + 2 ^ eoff); [|omega].
-      rewrite sum_of_concat, Z.add_comm; f_equal.
-      f_equal. 
-      rewrite Nat.sub_add_distr, <-le_plus_minus; auto.
-      destruct kix; simpl; try omega; rewrite mult_comm; simpl. generalize (kix * (2 ^ eoff + 2 ^ eoff)); intros; omega.
-    + cutrewrite (min (2 ^ rdiv2 (ix + 1)) offset = min (2 ^ rdiv2 (ix + 1)) (offset * 2)); auto.
+    sep_rewrite_in (ls_exists0 0 (n := ntrd)) H; auto; destruct H as [offsets H]; sep_split_in H.
+    sep_rewrite_in (ls_exists0 0 (n := ntrd)) H; auto; destruct H as [ds H]; sep_split_in H.
+    sep_rewrite_in (ls_exists0 (fun _ : nat => 0%Z) (n := ntrd)) H; auto; destruct H as [fcs H]; sep_split_in H.
+    repeat sep_rewrite_in (@ls_star ntrd) H.
+    repeat sep_rewrite_in (@ls_pure ntrd) H; sep_split_in H.
+    
+    Lemma vars_eq0 s (E : exp) len (f : nat -> nat) :
+      len <> 0 ->
+      conj_xs (ls_init 0 len (fun i => (E === Zn (f i)))) s emp_ph -> 
+      exists v, forall i, i < len -> f i = v.
+    Proof.
+      intros Hlen Hconj; exists (f 0); intros i Hil; destruct i; simpl; auto.
+      pose proof (@ls_emp _ _ 0 Hconj) as H0; rewrite ls_init_spec in H0; destruct lt_dec; try omega.
+      pose proof (@ls_emp _ _ (S i) Hconj) as HS; rewrite ls_init_spec in HS; destruct lt_dec; try omega.
+      unfold_pures. rewrite HS in H0; apply Nat2Z.inj in H0; auto.
+    Qed.
+    destruct ntrd_is_p2 as [e Hen].
+    assert (ntrd <> 0) by (pose proof (Nat.pow_nonzero 2 e); omega).
+    
+    pose proof (vars_eq0 s Offset ntrd _  H0 HP2) as [offset Hoff]; auto.
+    pose proof (vars_eq0 s D ntrd _  H0 HP3) as [d Hd]; auto.
+    
+    pose proof (@ls_emp _ _ 0 HP4) as Hdof; rewrite ls_init_spec in Hdof; simpl in Hdof.
+    destruct (lt_dec 0 ntrd); try omega.
+    rewrite Hoff, Hd in Hdof; try omega.
+
+    pose proof (@ls_emp _ _ 0 HP5) as Hd0; rewrite ls_init_spec in Hd0; simpl in Hd0.
+    destruct (lt_dec 0 ntrd); try omega.
+    rewrite Hd in Hd0; try omega.
+
+    unfold_pures.
+    destruct Hdof as [| Hdof]; try omega.
+    
+    erewrite ls_init_eq0 in H; [|intros; rewrite Hd, Hoff; auto; reflexivity].
+    
+    sep_rewrite (ls_exists0 0 (n:=ntrd)); auto; exists offsets; sep_split; auto.
+    sep_rewrite (ls_exists0 0 (n:=ntrd)); auto; exists ds; sep_split; auto.
+    set (fc' := fun i =>
+                  (nth (i / Nat.max 2 offset) fcs (fun _:nat=>0%Z)) i).
+    sep_rewrite (ls_exists0 (fun _:nat => 0%Z) (n:=ntrd)); auto; exists (nseq ntrd fc'); sep_split.
+    rewrite length_nseq; unfold_conn; auto.
+
+    repeat sep_rewrite (@ls_star ntrd). 
+    repeat sep_rewrite (@ls_pure ntrd).
+    repeat sep_split; auto.
+
+    rewrite <-(firstn_skipn (d * 2) (ls_init _ _ _)) in H.
+    rewrite firstn_init, skipn_init in H.
+    apply conj_xs_app in H.
+    lazymatch type of H with
+    | ((_ ** conj_xs (ls_init ?b ?n ?P)) _ _) =>
+      evar (fc : nat -> assn); 
+        sep_rewrite_in (@ls_init_eq' _ P fc n b) H; unfold fc in *
+    end.
+    Focus 2.
+    intros i Hi; destruct lt_dec; try omega.
+    instantiate (1 := fun _ => emp); reflexivity.
+    sep_rewrite_in init_emp_emp H; sep_normal_in H.
+    
+    erewrite ls_init_eq0 in H.
+    Focus 2.
+    { intros; destruct lt_dec; rewrite Nat.min_glb_lt_iff in H1; try omega; reflexivity. } Unfocus.
+    sep_rewrite_in (@ls_star) H; sep_rewrite_in (@ls_pure) H; sep_split_in H.
+
+    sep_rewrite (@ls_init_eq0).
+    Focus 2.
+    { intros i Hi; rewrite Hd, Hoff; auto; reflexivity. } Unfocus.
+    rewrite <-(firstn_skipn (d) (ls_init _ _ _)).  
+    rewrite firstn_init, skipn_init; apply conj_xs_app.
+    lazymatch goal with
+    | [|- ((_ ** conj_xs (ls_init ?b ?n ?P)) _ _)] =>
+      evar (Q : nat -> assn); 
+        sep_rewrite (@ls_init_eq' _ P Q n b); unfold Q in *
+    end.
+    Focus 2.
+    { intros; destruct lt_dec; try omega.
+      instantiate (1 := fun _ : nat => emp); reflexivity. } Unfocus.
+    sep_rewrite init_emp_emp; sep_normal.
+    assert (d <= ntrd).
+    { destruct offset; simpl in Hdof; try omega.
+      rewrite mult_comm in Hdof; simpl in Hdof.
+      generalize (offset * d) Hdof; intros; try omega. } 
+    rewrite Min.min_l; eauto.
+
+    sep_rewrite @ls_init_eq0; [|intros; destruct lt_dec; try omega; reflexivity].
+    assert (0 < offset).
+    { destruct offset; rewrite mult_comm in Hdof; simpl in Hdof; try omega. }
+    sep_rewrite (@ls_star); sep_rewrite (@ls_pure); sep_split.
+    - apply ls_emp'; rewrite init_length; intros i Hid; rewrite ls_init_spec; destruct lt_dec; 
+      [| unfold TrueP; eauto].
+      unfold_conn; intros j Hjn; rewrite nth_nseq; destruct (lt_dec (i+0) ntrd); try omega.
+      destruct (leb ntrd (0 + i)) eqn:Hni; [apply leb_iff in Hni; omega|].
+      unfold fc'.
+      
+      apply (ls_emp _ _ (j / Nat.max 2 offset)) in HP6; rewrite ls_init_spec in HP6.
+      assert (0 < Nat.max 2 offset).
+      { unfold Nat.max; destruct (Nat.max_dec 2 offset) as [Heq | Heq]; rewrite Heq; try omega. }
+      assert (d * 2 <= ntrd \/ ntrd < d * 2) as [Hd2n | Hd2n] by omega.
+      + rewrite Nat.min_l in HP6; eauto.
+        assert (j / (Nat.max 2 offset) < d * 2).
+        { apply Nat.div_lt_upper_bound; try omega.
+          rewrite Nat.max_comm.
+          destruct (Nat.max_spec offset 2).
+          destruct H4; unfold Nat.max; rewrite H5.
+          assert (offset = 1) by omega.
+          rewrite H6 in Hdof; try omega.
+          destruct H4; unfold Nat.max; rewrite H5.
+          rewrite mult_assoc, (mult_comm offset d); rewrite Hdof; eauto. }
+        destruct lt_dec; try omega.
+        unfold_pures; apply (HP6 j); eauto.
+      + rewrite Nat.min_r in HP6; try omega.
+        assert (offset < 2).
+        rewrite <-Hdof in Hd2n; apply Nat.mul_lt_mono_pos_l in Hd2n; eauto.
+        rewrite Nat.max_l in *; try omega.
+        assert (j / 2 < ntrd) by (apply Nat.div_lt_upper_bound; omega).
+        destruct lt_dec; try omega.
+        apply HP6; eauto.
+    - assert (offset < 2 \/ 2 <= offset) as [Ho2 | Ho2] by omega.
+      + assert (offset = 1) as Ho1 by omega.
+        assert (d = ntrd) as Hdn by (rewrite Ho1 in Hdof; omega).
+        unfold fc'; subst d offset.
+        rewrite Nat.max_l in *; try omega.
+        rewrite Nat.min_r in H; try omega.
+
+        Lemma is_array_conj (e : exp) (n : nat) 
+          
+        
+      Focus 2.
+      { intros i Hid.
+        rewrite nth_nseq; destruct (leb ntrd i) eqn:Heq.
+        apply leb_iff in Heq; omega.
+        reflexivity. } Unfocus.
+      
+      sep_rewrite_in_r (@equiv_from_nth emp (ls_init 0 (min (d * 2) ntrd) (fun i : nat =>
+            is_array Sum (Nat.max 2 offset) fc' (i * Nat.max 2 offset)))) H;
+        try (rewrite !init_length; auto).
+      Focus 2.
+      intros i Hi stc.
+      rewrite !ls_init_spec; destruct lt_dec; try omega; simpl.
+      apply is_array_change.
+      intros x Hx; unfold fc'.
+      pose proof (ls_emp _ _ i HP6) as HP8; rewrite ls_init_spec in HP8.
+      destruct lt_dec; try omega.
+      unfold_conn_in HP8; simpl in HP8.
+      rewrite HP8.
+      Focus 2.
+      { assert (offset < 2 \/ 2 <= offset) as [Ho2 | Ho2] by omega.
+        - assert (offset = 1) by omega; subst offset.
+          rewrite <-Hdof; unfold Nat.max; simpl.
+          rewrite <-Hdof in Hi; rewrite Min.min_r in Hi; try omega.
+          unfold Nat.max in Hx; simpl in Hx.
+          omega. 
+        - rewrite Nat.max_r; try omega.
+          assert (d * 2 <= ntrd).
+          rewrite <-Hdof; apply mult_le_compat_l; try omega.
+          rewrite Nat.min_l in Hi; try omega.
+          rewrite Nat.max_r in Hx; try omega.
+          rewrite <-Hdof.
+          unfold lt in Hi.
+          assert (i * offset + offset <= d * offset * 2).
+          { rewrite (Nat.mul_le_mono_pos_r _ _ offset) in Hi; try omega.
+            simpl in Hi.
+            cutrewrite (d * offset * 2 = d * 2 * offset); [|ring].
+            omega. }
+          generalize (i * offset) (d * offset *2 )H4; intros. omega. } Unfocus.
+          
+      assert ((x + i * Nat.max 2 offset) / Nat.max 2 offset < min (d * 2) ntrd).
+      { rewrite Nat.div_add.
+        rewrite Nat.div_small; try omega.
+        assert (offset < 2 \/ 2 <= offset) as [Hol | Hol] by omega.
+        rewrite Nat.max_l; omega.
+        rewrite Nat.max_r; omega. }
+      pose proof (ls_emp _ _ ((x + i * Nat.max 2 offset) / Nat.max 2 offset) HP6) as HP9.
+      rewrite ls_init_spec in HP9; destruct lt_dec.
+      unfold_conn_in HP7; rewrite HP7; try omega.
+      pose proof (ls_emp _ _ i HP6) as HP8; rewrite ls_init_spec in HP8.
+      destruct lt_dec; try omega.
+      unfold_conn_in HP8. simpl in HP8.
+
       
 Definition downsweep :=
   D ::= 1 ;;
